src/proof/index.v
@@ -10,7 +10,7 @@ Context `{!auth_setG Σ KKey.t}.
 
 (* TODO: revisit this spec *)
 Lemma wp_State__ByIndex_pod γ l kind index_name indexed_value
-  parent_key owned_parent owned_pod_map owned_child_keys:
+  parent_key owned_parent pod_map owned_child_keys:
   {{{ is_pkg_init apimodel ∗
       "#Hisk" ∷ is_kubernetes γ l ∗
       "%Hkind" ∷ ⌜ kind = "Pod"%go ⌝ ∗
@@ -20,23 +20,25 @@ Lemma wp_State__ByIndex_pod γ l kind index_name indexed_value
                                             parent_key.(KKey.Name') ++ "/"%go ++
                                             (PureKObject.metadata owned_parent).(PureObjectMeta.UID') ⌝ ∗
       "Hown_parent" ∷ parent_key [[ γ.(γ_state) ]]↦ owned_parent ∗
-      "Hown_pods" ∷ ([∗ map] key ↦ pod ∈ owned_pod_map, key [[ γ.(γ_state) ]]↦ PureKObject.Pod pod) ∗
+      "Hown_pod_list" ∷ ([∗ map] key ↦ pod ∈ pod_map, key [[ γ.(γ_state) ]]↦ PureKObject.Pod pod) ∗
       "Hown_child_keys" ∷ parent_key [[ γ.(γ_children) ]]↦ owned_child_keys ∗
-      "%Hdom_eq" ∷ ⌜ owned_child_keys = dom owned_pod_map ⌝
+      "%Hdom_eq" ∷ ⌜ owned_child_keys = dom pod_map ⌝
   }}}
     l @ (ptrT.id apimodel.State.id) @ "ByIndex" #kind #index_name #indexed_value
-  {{{ objs_l (ptrs: list loc) (pods: list v1.Pod.t) (pure_pods: list PurePod.t) dq, RET (#objs_l, #interface.nil);
-      "Hobjs_l" ∷ objs_l ↦* map (λ ptr, interface.mk (ptrT.id v1.Pod.id) #ptr) ptrs∗
-      "Hptrs_pods" ∷ ([∗ list] ptr;pod ∈ ptrs;pods, ptr ↦{dq} pod) ∗
-      "Hpods_purepods" ∷ ([∗ list] pod;pure_pod ∈ pods;pure_pods, PurePod.deepown pod pure_pod dq) ∗
-      "%Hwell_formed_pure_pods" ∷ ⌜ ∀ pure_pod, pure_pod ∈ pure_pods → PurePod.well_formed pure_pod ⌝ ∗
-      "%Hlen_pure_pods" ∷ ⌜ length pure_pods = size owned_pod_map ⌝ ∗
-      "%Hkey_set_equal_dom_owned_pods" ∷  ⌜ ∀ pure_pod, pure_pod ∈ pure_pods → ∃ k, owned_pod_map !! k = Some pure_pod ⌝ ∗
+  {{{ objs_l (ptr_list: list loc) (pod_list: list v1.Pod.t) (pure_pod_list: list PurePod.t) dq, RET (#objs_l, #interface.nil);
+      "Hobjs_l" ∷ objs_l ↦* map (λ ptr, interface.mk (ptrT.id v1.Pod.id) #ptr) ptr_list∗
+      "Hptrs_pods" ∷ ([∗ list] ptr;pod ∈ ptr_list;pod_list, ptr ↦{dq} pod) ∗
+      "Hpods_purepods" ∷ ([∗ list] pod;pure_pod ∈ pod_list;pure_pod_list, PurePod.deepown pod pure_pod dq) ∗
+      "%Hwell_formed_pure_pod_list" ∷ ⌜ ∀ p, p ∈ pure_pod_list → PurePod.well_formed p ⌝ ∗
+      "%Hlen_size_eq" ∷ ⌜ length pure_pod_list = size pod_map ⌝ ∗
+      "%Hlist_in_map" ∷  ⌜ ∀ p, p ∈ pure_pod_list → pod_map !! (PurePod.key p) = Some p ⌝ ∗
+      "%Hmap_in_list" ∷ ⌜ ∀ k p, pod_map !! k = Some p → p ∈ pure_pod_list ⌝ ∗
+      "%Hown_pod_keys_eq" ∷ ⌜ ∀ key pod, pod_map !! key = Some pod → key = PurePod.key pod ⌝ ∗
+      "%Hown_pod_list_namespace_eq" ∷ ⌜ ∀ key, key ∈ dom pod_map → key.(KKey.Namespace') = parent_key.(KKey.Namespace') ⌝ ∗
+      "%Hno_dup" ∷ ⌜ ∀ i j p1 p2, i ≠ j → pure_pod_list !! i = Some p1 → pure_pod_list !! j = Some p2 → (PurePod.key p1) ≠ (PurePod.key p2) ⌝ ∗
       "Hown_parent" ∷ parent_key [[ γ.(γ_state) ]]↦ owned_parent ∗
-      "Hown_pods" ∷ ([∗ map] key ↦ pod ∈ owned_pod_map, key [[ γ.(γ_state) ]]↦ PureKObject.Pod pod) ∗
-      "Hown_child_keys" ∷ parent_key [[ γ.(γ_children) ]]↦ owned_child_keys ∗
-      "%Hown_pod_keys_eq" ∷ ⌜ ∀ key pod, owned_pod_map !! key = Some pod → key = PurePod.key pod ⌝ ∗
-      "%Hown_pods_namespace_eq" ∷ ⌜ ∀ key, key ∈ dom owned_pod_map → key.(KKey.Namespace') = parent_key.(KKey.Namespace') ⌝
+      "Hown_pod_list" ∷ ([∗ map] key ↦ pod ∈ pod_map, key [[ γ.(γ_state) ]]↦ PureKObject.Pod pod) ∗
+      "Hown_child_keys" ∷ parent_key [[ γ.(γ_children) ]]↦ owned_child_keys
   }}}.
 Proof.
 Admitted.
