src/proof/k8s_io/apimachinery/pkg/api/errors.v
@@ -1,0 +1,18 @@
+From New.proof.k8s_io.apimachinery.pkg.api Require Export errors_init.
+From New.proof Require Import prelude empty_ffi.
+
+Section proof.
+Context `{hG: !heapGS Σ} {go_ctx: GoContext}.
+
+Lemma wp_IsNotFound_nil err:
+  {{{ is_pkg_init code.k8s_io.apimachinery.pkg.api.errors.errors ∗
+      ⌜ err = interface.nil ⌝
+  }}}
+    @! errors.IsNotFound #err
+  {{{ RET (#false);
+    True%I
+  }}}.
+Proof.
+Admitted.
+
+End proof.
