src/proof/util.v
@@ -1,0 +1,93 @@
+From New.proof Require Import prelude empty_ffi.
+From New.proof Require Export pure_objects.
+
+Section proof.
+Context `{hG: !heapGS Σ} {go_ctx: GoContext}.
+
+Lemma filter_preserves_key_uniqueness {A} (key : A → KKey.t) (P : A → Prop) `{∀ x, Decision (P x)} (xs : list A) :
+  (∀ i j x y, i ≠ j → xs !! i = Some x → xs !! j = Some y → key x ≠ key y) →
+  (∀ i j x y, i ≠ j → filter P xs !! i = Some x → filter P xs !! j = Some y → key x ≠ key y).
+Proof.
+  intros Hno_dup i j x y Hneq Hi Hj Hkeys_eq.
+  assert (x = y) as Heq.
+  { apply list_elem_of_lookup_2 in Hi as Hi'. apply list_elem_of_filter in Hi' as [_ Hi_in].
+    apply list_elem_of_lookup_2 in Hj as Hj'. apply list_elem_of_filter in Hj' as [_ Hj_in].
+    apply list_elem_of_lookup_1 in Hi_in as [i_orig Hi_orig].
+    apply list_elem_of_lookup_1 in Hj_in as [j_orig Hj_orig].
+    destruct (decide (i_orig = j_orig)) as [|].
+    - subst j_orig. congruence.
+    - exfalso. apply (Hno_dup i_orig j_orig x y); done. }
+  subst y.
+  assert (NoDup xs) as HNoDup.
+  { apply NoDup_alt. intros i' j' x' Hi' Hj'.
+    destruct (decide (i' = j')) as [|]; [done|].
+    exfalso. apply (Hno_dup i' j' x' x'); done. }
+  assert (NoDup (filter P xs)) as HNoDup_filtered.
+  { apply list.NoDup_filter. done. }
+  assert (i = j) by (eapply NoDup_lookup; eauto).
+  done.
+Qed.
+
+Lemma filter_list_map_size_eq {K V} `{FinMap K M} (key_fn : V → K) (P : V → Prop) `{∀ v, Decision (P v)} (xs : list V) (m : M V) :
+  (* Every element in xs appears in m with the right key *)
+  (∀ x, x ∈ xs → m !! key_fn x = Some x) →
+  (* Every element in m appears in xs (surjectivity) *)
+  (∀ k v, m !! k = Some v → v ∈ xs) →
+  (* Keys are canonical: if m maps k to v, then k = key_fn v *)
+  (∀ k v, m !! k = Some v → k = key_fn v) →
+  (* xs has no duplicate keys *)
+  (∀ i j x y, i ≠ j → xs !! i = Some x → xs !! j = Some y → key_fn x ≠ key_fn y) →
+  (* Same size before filtering *)
+  length xs = size m →
+  (* Then filtering by compatible predicates yields same size *)
+  length (filter P xs) = size (filter (λ kv, P kv.2) m).
+Proof.
+  intros Hin Hmap_in_list Hkey_eq Hno_dup Hlen_size_eq.
+  rewrite map_filter_alt.
+  assert (NoDup (filter (λ kv, P kv.2) (map_to_list m)).*1) as HNoDup_filtered.
+  { cut (∀ l : list (K * V), NoDup l.*1 → NoDup (filter (λ kv, P kv.2) l).*1).
+    { intro Hcut. apply Hcut. apply NoDup_fst_map_to_list. }
+    clear. intros l. induction l as [|[k v] rest IH]; intro HNoDup; simpl.
+    - done.
+    - rewrite filter_cons. case_decide; simpl.
+      + constructor.
+        * intros Hin_k. apply NoDup_cons_1_1 in HNoDup.
+          assert (k ∈ rest.*1) by
+            (clear -Hin_k; induction rest as [|[k' v'] rest' IH']; [inversion Hin_k|];
+             rewrite filter_cons in Hin_k; case_decide; simpl in Hin_k;
+             [apply elem_of_cons in Hin_k as [->|Hin_k]; [left|right; apply IH']; done
+             |right; apply IH'; done]).
+          done.
+        * apply IH. by apply NoDup_cons_1_2 in HNoDup.
+      + apply IH. by apply NoDup_cons_1_2 in HNoDup. }
+  rewrite (map_size_list_to_map _ HNoDup_filtered).
+  assert ((filter (λ kv, P kv.2) (map_to_list m)).*2 ≡ₚ filter P xs) as Hperm.
+  { apply NoDup_Permutation.
+    - apply NoDup_fmap_2_strong.
+      + intros [k1 v1] [k2 v2] Hin1 Hin2. simpl. intros <-.
+        apply list_elem_of_filter in Hin1 as [_ Hin1].
+        apply list_elem_of_filter in Hin2 as [_ Hin2].
+        apply elem_of_map_to_list in Hin1, Hin2.
+        assert (k1 = key_fn v1) as -> by (apply Hkey_eq; done).
+        assert (k2 = key_fn v1) as -> by (apply Hkey_eq; done).
+        done.
+      + apply list.NoDup_filter, NoDup_map_to_list.
+    - apply list.NoDup_filter, NoDup_alt. intros i j x Hi Hj.
+      destruct (decide (i = j)); [done|exfalso; eapply Hno_dup; eauto].
+    - intros v. split.
+      + intros Hv. apply list_elem_of_fmap_1 in Hv as [kv [Heq Hkv]].
+        destruct kv as [k v']. simpl in Heq. subst v'.
+        apply list_elem_of_filter in Hkv as [HPkv Hkv].
+        apply list_elem_of_filter. split; [done|].
+        by apply elem_of_map_to_list, Hmap_in_list in Hkv.
+      + intros Hv. apply list_elem_of_filter in Hv as [HPv Hv_in].
+        apply Hin in Hv_in as Hlookup.
+        change v with ((key_fn v, v).2).
+        apply (list_elem_of_fmap_2 snd).
+        apply list_elem_of_filter. split; [simpl; done|].
+        apply elem_of_map_to_list. done. }
+  rewrite -(Permutation_length Hperm).
+  apply length_fmap.
+Qed.
+
+End proof.
